Support incomplete types in typedefs.

tests/defined/incomplete_typedef.c
@@ -1,0 +1,7 @@
+typedef struct S T;
+struct S { int x; };
+
+int main() {
+  T s; s.x = 10;
+  return s.x;
+}
